steel/Zeta.Steel.LogEntry.fsti
@@ -3,10 +3,28 @@ include Zeta.Steel.LogEntry.Spec
 open Zeta.Steel.Parser
 module U32 = FStar.UInt32
 
-val parser_log_entry : parser spec_parser_log_entry
+val zeta__parser_log_entry : parser spec_parser_log_entry
 
-val serialize_stamped_record : serializer spec_serializer_stamped_record
+inline_for_extraction
+noextract
+let parser_log_entry : parser spec_parser_log_entry = zeta__parser_log_entry
 
-val serialize_value : serializer spec_serializer_value
+val zeta__serialize_stamped_record : serializer spec_serializer_stamped_record
 
-val parser_u256 : parser spec_parser_u256
+inline_for_extraction
+noextract
+let serialize_stamped_record : serializer spec_serializer_stamped_record = zeta__serialize_stamped_record
+
+inline_for_extraction
+noextract
+val zeta__serialize_value : serializer spec_serializer_value
+
+inline_for_extraction
+noextract
+let serialize_value : serializer spec_serializer_value = zeta__serialize_value
+
+val zeta__parser_u256 : parser spec_parser_u256
+
+inline_for_extraction
+noextract
+let parser_u256 : parser spec_parser_u256 = zeta__parser_u256
