steel/formats/lowstar/Zeta.LowStar.LogEntry.fsti
@@ -2,10 +2,10 @@ module Zeta.LowStar.LogEntry
 open Zeta.Steel.LogEntry.Spec
 open Zeta.LowStar.Parser
 
-val parser_log_entry : parser spec_parser_log_entry
+val zeta__parser_log_entry : parser spec_parser_log_entry
 
-val serialize_stamped_record : serializer spec_serializer_stamped_record
+val zeta__serialize_stamped_record : serializer spec_serializer_stamped_record
 
-val serialize_value : serializer spec_serializer_value
+val zeta__serialize_value : serializer spec_serializer_value
 
-val parser_u256 : parser spec_parser_u256
+val zeta__parser_u256 : parser spec_parser_u256
